"same start address and same size" does not imply "safe to cancel"
because the clause to be canceled could be a bst node with different
subtrees than the candidate clause.
Stronger condition: both clauses need to be contiguous (which implies
that they have no pointers to other memory that might differ) OR
cancelling the clause with the candidate clause works right away
(without splitting it into steps and potentially leaving some subgoals
open for manual proving, which requires knowing that the cancellation
decision is safe).

bedrock2/src/bedrock2/to_from_anybytes.v
@@ -2,6 +2,7 @@ Require Import Coq.ZArith.ZArith. Local Open Scope Z_scope.
 Require Import Coq.micromega.Lia.
 Require Import coqutil.Word.Interface coqutil.Word.Properties coqutil.Word.Bitwidth.
 Require Import coqutil.Map.Interface.
+Require Import coqutil.Tactics.Tactics.
 Require Import coqutil.Datatypes.ZList. Import ZList.List.ZIndexNotations.
 Require Import bedrock2.Lift1Prop bedrock2.Map.Separation bedrock2.Map.SeparationLogic.
 Require Import bedrock2.SepLib.
@@ -13,6 +14,14 @@ Section WithMem.
 
   Definition contiguous(P: word -> mem -> Prop)(n: Z): Prop :=
     forall addr, impl1 (P addr) (array (uint 8) n ? addr).
+
+  (* sometimes, we don't need the actual proof, but only want to know whether it's
+     contiguous to determine whether a proof step is safe, so we can save the proof effort *)
+  Inductive fake_contiguous(P: word -> mem -> Prop): Prop :=
+    mk_fake_contiguous.
+
+  Lemma contiguous_to_fake P n: contiguous P n -> fake_contiguous P.
+  Proof. intros. constructor. Qed.
 
   Lemma cast_to_anybytes: forall (P: word -> mem -> Prop) a n m,
       contiguous P n -> P a m -> (array (uint 8) n ? a) m.
@@ -80,6 +89,20 @@ Section WithMem.
     assumption.
   Qed.
 
+  Lemma uint_contiguous: forall (nbits v: Z),
+      contiguous (uint nbits v) (nbits_to_nbytes nbits).
+  Proof.
+    unfold contiguous, impl1. intros nbits v addr m H. eapply anybytes_from_alt.
+    { apply nbits_to_nbytes_nonneg. }
+    unfold uint in H. eapply sep_emp_l in H. apply proj2 in H.
+    unfold Scalars.littleendian, ptsto_bytes.ptsto_bytes in H.
+    rewrite HList.tuple.to_list_of_list in H.
+    eapply Array.array_1_to_anybytes in H.
+    rewrite LittleEndianList.length_le_split in H.
+    rewrite Z2Nat.id in H by apply nbits_to_nbytes_nonneg.
+    exact H.
+  Qed.
+
   Lemma uintptr_fillable: fillable uintptr (Memory.bytes_per_word width).
   Proof.
     unfold fillable, iff1, uintptr. intros a m. split; intro Hm.
@@ -88,6 +111,27 @@ Section WithMem.
       eapply anybytes_from_alt. 2: exact Hm.
       destruct width_cases as [E|E]; rewrite E; cbv; discriminate.
   Qed.
+
+  (* TODO make non-fake *)
+  Lemma array_fake_contiguous: forall T (elem: T -> word -> mem -> Prop)
+                                      {sz: PredicateSize elem} n vs,
+      (forall v, fake_contiguous (elem v)) ->
+      fake_contiguous (array elem n vs).
+  Proof. intros. constructor. Qed.
+
+  Lemma sepapps_nil_fake_contiguous: fake_contiguous (sepapps nil).
+  Proof. constructor. Qed.
+
+  Lemma sepapps_cons_fake_contiguous: forall p sz l,
+      fake_contiguous p ->
+      fake_contiguous (sepapps l) ->
+      fake_contiguous (sepapps (cons (mk_sized_predicate p sz) l)).
+  Proof. intros. constructor. Qed.
+
+  Lemma anyval_fake_contiguous{T: Type}: forall p: T -> word -> mem -> Prop,
+      (forall v, fake_contiguous (p v)) ->
+      fake_contiguous (anyval p).
+  Proof. intros. constructor. Qed.
 End WithMem.
 
 Section WithMem32.
@@ -118,7 +162,13 @@ Create HintDb contiguous.
   sepapps_nil_contiguous
   uintptr32_contiguous
   uintptr64_contiguous
+  uint_contiguous
   anybytes_contiguous
+  contiguous_to_fake
+  array_fake_contiguous
+  sepapps_nil_fake_contiguous
+  sepapps_cons_fake_contiguous
+  anyval_fake_contiguous
 : contiguous.
 
 Create HintDb fillable.
@@ -126,3 +176,42 @@ Create HintDb fillable.
   uintptr32_fillable
   uintptr64_fillable
 : fillable.
+
+#[export] Hint Extern 20 (contiguous ?p ?n) =>
+  let h := head p in
+  (* seemingly superfluous match strips cast added by unfold *)
+  lazymatch constr:(ltac:(unfold h; typeclasses eauto) : contiguous p n) with
+  | ?res => exact res
+  end
+: contiguous.
+
+Ltac is_contiguous P :=
+  let __ := constr:(ltac:(solve [typeclasses eauto with contiguous]
+                          || fail "not contiguous")
+                     : contiguous P _) in idtac.
+
+Ltac is_fake_contiguous P :=
+  let __ := constr:(ltac:(solve [typeclasses eauto with contiguous]
+                          || fail "not fake_contiguous")
+                     : fake_contiguous P) in idtac.
+
+Section TestsWithMem64.
+  Context {word: word 64} {BW: Bitwidth 64} {mem: map.map word Byte.byte}
+          {word_ok: word.ok word} {mem_ok: map.ok mem}.
+
+  Goal forall (foo: word -> mem -> Prop) (v: word), True.
+    intros.
+    is_contiguous (uintptr v).
+    Fail is_contiguous foo.
+    Fail is_fake_contiguous foo.
+    assert (fake_contiguous foo) as A.
+    2: {
+      Fail is_contiguous foo.
+      is_fake_contiguous foo.
+      clear A.
+      assert (contiguous foo 42) as A.
+      2: {
+        is_contiguous foo.
+        is_fake_contiguous foo.
+  Abort.
+End TestsWithMem64.
