LiveVerif/src/LiveVerifExamples/ErrorTests/safe_f_equal_errors.v
@@ -3,6 +3,35 @@ Require Import LiveVerif.LiveVerifLib.
 
 Load LiveVerif.
 
+Variable foo: word -> word -> mem -> Prop.
+
+Goal forall (p v1 v2: word) R (m' m1 m: mem),
+    m1 |= R ->
+    mmap.du m1 m = m' ->
+    m |= foo v1 p ->
+  <{ * foo v2 p
+     * R }> m'.
+Proof.
+  intros. steps.
+  lazymatch goal with
+  | _: warning_marker (PredicateSize_not_found (foo _)) |- _ => idtac
+  end.
+Abort.
+
+#[local] Hint Extern 1 (PredicateSize foo) => exact 4 : typeclass_instances.
+
+Goal forall (p v1 v2: word) R (m' m1 m: mem),
+    m1 |= R ->
+    mmap.du m1 m = m' ->
+    m |= foo v1 p ->
+  <{ * foo v2 p
+     * R }> m'.
+Proof.
+  intros. steps.
+  test_error Error:("Cannot cancel" (foo v2 p) "with" (foo v1 p)
+                      "even though both span the same range:" 4 "bytes from" p).
+Abort.
+
 Goal forall n l (i j count p: word) R (m' m1 m: mem),
     m1 |= R ->
     mmap.du m1 m = m' ->
