bedrock2/src/bedrock2/syntactic_f_equal_with_ZnWords.v
@@ -1,0 +1,18 @@
+Require Import Coq.ZArith.ZArith.
+Require Import coqutil.Word.Interface.
+Require Import bedrock2.ZnWords.
+Require Import bedrock2.Lift1Prop.
+
+Lemma f_equal_fun[A B: Type]: forall (f g: A -> B) (x: A), f = g -> f x = g x.
+Proof. intros. subst. reflexivity. Qed.
+
+Ltac syntactic_f_equal_step_with_ZnWords :=
+  lazymatch goal with
+  | |- ?x = ?x => reflexivity
+  | |- @eq (@word.rep _ _) _ _ => ZnWords
+  | |- @eq Z _ _ => ZnWords
+  | |- ?f ?a = ?f ?b => eapply (@f_equal _ _ f a b)
+  | |- ?f ?x = ?g ?x => eapply (f_equal_fun f g x)
+  end.
+
+Ltac syntactic_f_equal_with_ZnWords := solve [repeat syntactic_f_equal_step_with_ZnWords].
